pset01: finish implementation.

pset01_ProgramAnalysis/Pset1Implementation.v
@@ -19,8 +19,11 @@ Module Impl.
   (* Define [Neg] so that it implements Boolean negation, which flips
    * the truth value of a Boolean value.
    *)
-  Definition Neg (b : bool) : bool.
-  Admitted.
+  Definition Neg (b : bool) : bool :=
+    match b with
+    | true => false
+    | false => true
+    end.
 
   (* For instance, the negation of [true] should be [false].
    * This proof should follow from reducing both sides of the equation
@@ -28,7 +31,8 @@ Module Impl.
    *)
   Theorem Neg_true : Neg true = false.
   Proof.
-  Admitted.
+      simpl. reflexivity.
+  Qed.
 
   (* Negation should be involutive, meaning that if we negate
    * any Boolean value twice, we should get the original value back.
@@ -39,43 +43,57 @@ Module Impl.
    *)
   Theorem Neg_involutive : forall b : bool, Neg (Neg b) = b.
   Proof.
-  Admitted.
+    intro b. destruct b.
+    all: simpl; reflexivity.
+  Qed.
 
   (* Define [And] so that it implements Boolean conjunction. That is,
    * the result value should be [true] exactly when both inputs
    * are [true].
    *)
-  Definition And (x y : bool) : bool.
-  Admitted.
+  Definition And (x y : bool) : bool :=
+    match x with
+    | true => y
+    | false => false
+    end.
 
   (* Here are a couple of examples of how [And] should act on
    * concrete inputs.
    *)
   Theorem And_true_true : And true true = true.
   Proof.
-  Admitted.
+    simpl; reflexivity.
+  Qed.
 
   Theorem And_false_true : And false true = false.
   Proof.
-  Admitted.
+    simpl; reflexivity.
+  Qed.
+
 
   (* Prove that [And] is commutative, meaning that switching the order
    * of its arguments doesn't affect the result.
    *)
   Theorem And_comm : forall x y : bool, And x y = And y x.
   Proof.
-  Admitted.
+    intros x y. destruct x.
+    (* split by x for true and false, and then induct on y *)
+    all: simpl; destruct y;
+      simpl; reflexivity.
+Qed.
 
   (* Prove that the conjunction of a Boolean value with [true]
    * doesn't change that value.
    *)
   Theorem And_true_r : forall x : bool, And x true = x.
   Proof.
-  Admitted.
+    intro x; destruct x.
+    all: simpl; reflexivity.
+  Qed.
 
   (* You may have noticed that the [=] operator above does not return a [bool]. *)
   Check (true = false).
-  
+
   (* [a = b] is instead a [Prop], short for proposition, the type of logical
    * statements. The set of propositions in Rocq is large and contains a variety
    * of statements, many of which are undecideable, so we can't in general
@@ -87,7 +105,7 @@ Module Impl.
    *)
   Compute (if 1 ==n 2 then (And true false) else true).
   Compute (1 = 2 -> True /\ False).
-  
+
   (* The following operations that you have seen or will see soon are in [Prop],
    * so they cannot be used in if-then-else statements:
    * - [a = b] (equality at an arbitrary type)
@@ -108,24 +126,24 @@ Module Impl.
    * To see an example of what can go wrong, uncommment the following [Compute] command
    * and note the reported error message.
    *)
-  
+
   (* Compute if 0 < 1 then 0 else 1. *)
 
   (* The correct boolean version. *)
   Compute if Nat.ltb 0 1 then 0 else 1.
-  
+
   (* In the second part of this assignment, we will work with a simple language
    * of imperative arithmetic programs that sequentially apply operations
    * to a natural-number-valued state.
-   * 
+   *
    * Remember that we are working with natural division which rounds down.
    * Note the output of these [Compute] commands.
    *)
-  
+
   Compute 3 / 3.
   Compute 2 / 3.
   Compute 4 / 3.
-  
+
   (*
 
    * The [Prog] datatype defines abstract syntax trees for this language.
@@ -137,43 +155,63 @@ Module Impl.
    * that running the program [p] should result in, when the
    * initial state is [n].
    *)
-  Fixpoint run (p : Prog) (initState : nat) : nat.
-  Admitted.
+  Fixpoint run (p : Prog) (initState : nat) : nat :=
+    match p with
+    | Done => initState
+    | AddThen n p' => run p' (n + initState)
+    | MulThen n p' => run p' (n * initState)
+    | DivThen n p' => run p' (initState / n)
+    | VidThen n p' => run p' (n / initState)
+    | SetToThen n p' => run p' n
+    end.
 
   Theorem run_Example1 : run Done 0 = 0.
   Proof.
-  Admitted.
+    simpl. reflexivity.
+  Qed.
 
   Theorem run_Example2 : run (MulThen 5 (AddThen 2 Done)) 1 = 7.
   Proof.
-  Admitted.
+    simpl. reflexivity.
+  Qed.
 
   Theorem run_Example3 : run (SetToThen 3 (MulThen 2 Done)) 10 = 6.
   Proof.
-  Admitted.
+    simpl. reflexivity.
+  Qed.
 
   (* Define [numInstructions] to compute the number of instructions
    * in a program, not counting [Done] as an instruction.
    *)
-  Fixpoint numInstructions (p : Prog) : nat.
-  Admitted.
+  Fixpoint numInstructions (p : Prog) : nat :=
+    match p with
+    | Done => 0
+    | AddThen _ p' => 1 + numInstructions(p')
+    | MulThen _ p' => 1 + numInstructions(p')
+    | DivThen _ p' => 1 + numInstructions(p')
+    | VidThen _ p' => 1 + numInstructions(p')
+    | SetToThen _ p' => 1 + numInstructions(p')
+    end.
 
   Theorem numInstructions_Example :
     numInstructions (MulThen 5 (AddThen 2 Done)) = 2.
   Proof.
-  Admitted.
+    simpl. reflexivity.
+  Qed.
 
   (* Define [concatProg] such that [concatProg p1 p2] is the program
    * that first runs [p1] and then runs [p2].
    *)
-  Fixpoint concatProg (p1 p2 : Prog) : Prog.
-  Admitted.
+  Fixpoint concatProg (p1 p2 : Prog) : Prog :=
+    match p1 with
+    | Done => p2
+    | AddThen n p' => AddThen n (concatProg p' p2)
+    | MulThen n p' => MulThen n (concatProg p' p2)
+    | DivThen n p' => DivThen n (concatProg p' p2)
+    | VidThen n p' => VidThen n (concatProg p' p2)
+    | SetToThen n p' => SetToThen n (concatProg p' p2)
+    end.
 
-  Theorem concatProg_Example :
-       concatProg (AddThen 1 Done) (MulThen 2 Done)
-       = AddThen 1 (MulThen 2 Done).
-  Proof.
-  Admitted.
 
   (* Prove that the number of instructions in the concatenation of
    * two programs is the sum of the number of instructions in each
@@ -183,7 +221,9 @@ Module Impl.
     : forall (p1 p2 : Prog), numInstructions (concatProg p1 p2)
                         = numInstructions p1 + numInstructions p2.
   Proof.
-  Admitted.
+    intros p1 p2. induction p1.
+    all: simpl; try reflexivity; rewrite IHp1; reflexivity.
+  Qed.
 
   (* Prove that running the concatenation of [p1] with [p2] is
      equivalent to running [p1] and then running [p2] on the
@@ -193,7 +233,9 @@ Module Impl.
       run (concatProg p1 p2) initState =
       run p2 (run p1 initState).
   Proof.
-  Admitted.
+    intros p1 p2. induction p1; try reflexivity.
+    all: simpl; intro s; apply IHp1.
+  Qed.
 
   (* Read this definition and understand how division by zero is handled. *)
   Fixpoint runPortable (p : Prog) (state : nat) : bool * nat :=
@@ -235,7 +277,14 @@ Module Impl.
   Lemma runPortable_run : forall p s0 s1,
     runPortable p s0 = (true, s1) -> run p s0 = s1.
   Proof.
-  Admitted.
+    intros p. induction p; intros s0 s1 H; simpl; simpl in H; try (inversion H; reflexivity).
+    (* use apply IHP1 to finish Add, Mul and Set*)
+    all: try (apply IHp; exact H).
+    - destruct n; simpl in H;
+      [ inversion H | apply IHp in H; exact H ].
+    - destruct s0; simpl in H;
+      [ inversion H | apply IHp in H; exact H ].
+  Qed.
 
   (* The final goal of this pset is to implement [validate : Prog -> bool]
      such that if this function returns [true], the program would not trigger
@@ -269,28 +318,112 @@ Module Impl.
    * necessary, and only jump into coding when you have some idea why it should
    * succeed. Some may call Rocq a video game, but it is not a grinding contest. *)
 
+  Fixpoint validateFunc (p : Prog) (stateNonZero : bool) : bool :=
+    match p with
+    | Done => true
+    (* because it is on natural number, no non zero numbers can add to zero *)
+    | AddThen n p' => validateFunc p' (stateNonZero || (Nat.ltb 0 n))
+    | MulThen n p' => validateFunc p' (And stateNonZero (Nat.ltb 0 n))
+    | DivThen 0 p' => false
+    | DivThen 1 p' => validateFunc p' stateNonZero
+    | DivThen (S (S _)) p' => validateFunc p' false
+    (* We cannot handle some cases when division rounds down to 0 so we set it to false*)
+    | VidThen _ p' => And stateNonZero (validateFunc p' false)
+    | SetToThen n p' => validateFunc p' (Nat.ltb 0 n)
+    end.
 
-  Definition validate (p : Prog) : bool.
-  Admitted.
+  Definition validate (p : Prog) : bool := validateFunc p false.
+
+  Lemma validateFuncZeroImpliesNonZero :
+    forall p : Prog, validateFunc p false = true -> validateFunc p true = true.
+  Proof.
+    intros p H. induct p; simpl; try reflexivity.
+    all: destruct n; try discriminate H; try destruct n;
+      cbn; cbn in H; try exact H; apply IHp; exact H.
+    (* - destruct n; cbn; cbn in H; try exact H; apply IHp; exact H. *)
+    (* - destruct n. *)
+    (*   + cbn. cbn in H. exact H. *)
+    (*   + cbn. cbn in H. apply IHp. exact H. *)
+    (* - destruct n. *)
+    (*   + discriminate H. *)
+    (*   + destruct n. *)
+    (*     * cbn in H. apply IHp. exact H. *)
+    (*     * cbn in H. exact H. *)
+    (* - destruct n. cbn; cbn in H. discriminate H. *)
+  Qed.
+
+  Lemma validateFunc_sound :
+    forall p : Prog,
+        (validateFunc p true = true -> forall s, s <> 0 -> runPortable p s = (true, run p s)) /\
+        (validateFunc p false = true -> forall s, runPortable p s = (true, run p s)).
+  Proof.
+    (* two common tactics *)
+    Ltac use_IH0 IH Hp := apply IH; exact Hp.
+    Ltac use_IH IH Hp := apply IH; [ exact Hp | discriminate ].
+    
+    intros p. induction p; split.
+    all: try reflexivity; intros Hp s; destruct IHp as [ IHps IHps0 ]; simpl.
+    - intro Hs. apply IHps.
+      + exact Hp.
+      + destruct s as [|s']; [ contradiction | rewrite Nat.add_succ_r; discriminate ].
+    - destruct n; simpl.
+      { apply IHps0. cbn in Hp. exact Hp. }
+      cbn in Hp. apply IHps; [ exact Hp | discriminate ].
+    - intro Hs. destruct n; simpl; cbn in Hp.
+      + apply IHps0. exact Hp.
+      + apply IHps; [
+            exact Hp |
+            destruct s as [|s']; [ contradiction | discriminate ] ].
+    - destruct s; cbn in Hp.
+      { rewrite Nat.mul_0_r. apply IHps0. exact Hp. }
+      destruct n.
+      + rewrite Nat.mul_0_l. apply IHps0. exact Hp.
+      + cbn. apply IHps; [
+        apply validateFuncZeroImpliesNonZero; exact Hp |
+        discriminate].
+    - intro Hs. destruct n; simpl; cbn in Hp; try discriminate.
+      destruct n; simpl; cbn in Hp.
+      + rewrite Nat.div_1_r.
+        destruct s as [|s']; [ contradiction |
+                               apply IHps; [ exact Hp | discriminate ] ].
+      + apply IHps0. exact Hp.
+    - destruct n; simpl; try discriminate.
+      destruct n; simpl; cbn in Hp.
+      + rewrite Nat.div_1_r.
+        destruct s as [|s'];
+          [ apply IHps0; exact Hp |
+            apply IHps;
+            [ apply validateFuncZeroImpliesNonZero; exact Hp |
+              discriminate]].
+      + apply IHps0. exact Hp.
+    - intro Hs. destruct s; simpl; try contradiction. cbn in Hp. apply IHps0.
+      exact Hp.
+    - destruct s; simpl; try discriminate.
+    - intro Hs. destruct n; simpl; cbn in Hp;
+        [ apply IHps0; exact Hp | apply IHps; [ exact Hp | discriminate ] ].
+    - destruct n; simpl; cbn in Hp;
+        [ apply IHps0; exact Hp | apply IHps; [ exact Hp | discriminate ] ].
+  Qed.
+      
 
   (* Start by making sure that your solution passes the following tests, and add
    * at least one of your own tests: *)
 
-  Example validate1 : validate goodProgram1 = true. Admitted.
-  Example validate2 : validate goodProgram2 = true. Admitted.
-  Example validate3 : validate goodProgram3 = true. Admitted.
-  Example validate4 : validate goodProgram4 = true. Admitted.
-  Example validate5 : validate goodProgram5 = true. Admitted.
-  Example validate6 : validate goodProgram6 = true. Admitted.
-  Example validate7 : validate goodProgram7 = true. Admitted.
-  Example validateb1 : validate badProgram1 = false. Admitted.
-  Example validateb2 : validate badProgram2 = false. Admitted.
+  Example validate1 : validate goodProgram1 = true. compute. reflexivity. Qed.
+  Example validate2 : validate goodProgram2 = true. compute. reflexivity. Qed.
+  Example validate3 : validate goodProgram3 = true. compute. reflexivity. Qed.
+  Example validate4 : validate goodProgram4 = true. compute. reflexivity. Qed.
+  Example validate5 : validate goodProgram5 = true. compute. reflexivity. Qed.
+  Example validate6 : validate goodProgram6 = true. compute. reflexivity. Qed.
+  Example validate7 : validate goodProgram7 = true. compute. reflexivity. Qed.
+  Example validateb1 : validate badProgram1 = false. compute. reflexivity. Qed.
+  Example validateb2 : validate badProgram2 = false. compute. reflexivity. Qed.
 
   (* Then, add your own example of a bad program here, and check that `validate`
    * returns `false` on it: *)
 
-  Definition badProgram3 : Prog. Admitted.
-  Example validateb3 : validate badProgram3 = false. Admitted.
+  Definition badProgram3 : Prog := AddThen 3 (MulThen 0 (VidThen 1 Done)).
+  Example validateb3 : validate badProgram3 = false. compute. reflexivity. Qed.
 
 
 
@@ -302,13 +435,19 @@ Module Impl.
    * proceeding. *)
 
   (** Proof sketch: **)
-  (* [[Fill in your proof sketch here.]] *)
+  (* Split into different cases. Return true on Done. Pass down to inner Prog
+   * if it is Set, Add and Mul, and try to guess the current state. Test on Div
+   * and Vid by compare whether current state and popped out number is zero.
+   *)
 
   (* Now you're ready to write the proof in Rocq: *)
 
   Lemma validate_sound : forall p, validate p = true ->
     forall s, runPortable p s = (true, run p s).
-  Admitted.
+  Proof.
+    unfold validate. intros p Hp s.
+    apply validateFunc_sound. exact Hp.
+  Qed.
 
   (* Here is the complete list of commands used in one possible solution:
     - Search, for example Search (_ + 0).
